## Rules of Inference

![image](https://obsidian-img-studies.tsun1031.xyz/2024/10/07/f420db55b0f9acf6ae0e075e51a305b19ba28cdf50d29d385f7bb04572aa61ef.png)

![image](https://obsidian-img-studies.tsun1031.xyz/2024/10/07/bbc01b23e0dc4e985a2427df81c600793f99836cfa69283b7d34f765e7423dde.png)

![image](https://obsidian-img-studies.tsun1031.xyz/2024/10/07/198a728eed6f62d716f11f2ad33046aa841917ce22366782e36ef6e4e2372e0b.png)

## Proof by Contradiction

To prove a statement by contradiction, **start by assuming the opposite of what you would like to prove**. Then show that the consequences of this premise are impossible. This means that your original statement must be true.

## Proof by Contraposition

$$
p \implies q \equiv \neg q \implies \neg p
$$

Assume (NOT $q$), then (NOT $p$).

![](https://youtu.be/b-kFWP9a2tw)

## PNF: Prenex Normal Form

### Guidelines

- Use different variable name
- If exists operators other than $\vee$ or $\land$
- Make sure **none of quantifiers is negated**
- We can then apply rules 1-4
