Which of the following statements (in which $Z^+$ stands for the positive integers and $Z$ stands for all integers) is true and which is false? Don't forget to explain why.

---

> [!summary] Part A  
> $\forall z \in \mathbb{Z}^+ (z^2 + 6z + 10 > 20)$

$$
z^2 + 6z - 10 > 0
$$

$$
x = \left( \dfrac{-6 - \sqrt{76}}{2}  ,  \dfrac{-6 + \sqrt{76}}{2} \right)
$$

$$\forall z \in \mathbb{Z}^+ = \text{False}$$

> [!summary] Part B  
> $\forall z \in \mathbb{Z}, (z^2 - z \ge 0)$

$$
z^2 - z > 0 \Leftrightarrow z^2 - z = 0 \Leftrightarrow z(z - 1) = 0  \Leftrightarrow z \in \{0, 1\}
$$

$$(-\infty,0] \cup [1,+\infty)$$  
$$\forall z \in \mathbb{Z} = \text{True}$$

> [!summary] Part C  
> $\exists z \in \mathbb{Z}^+, (z - z^2 > 0)$

$$z(1 - z) \Leftrightarrow z = {0,-1}$$

$$x = (-1,0)$$

$$\exists z \in \mathbb{Z}^+ = \text{False}$$

> [!summary] Part D  
> $\exists z \in \mathbb{Z}, (z^2 - z = 6)$

$$z^2 - z - 6 = 0$$

$$z = \{3,-2\}$$

$$\exists z \in \mathbb{Z} = \text{True}$$
